Update heap.dfy

heap.dfy
@@ -4,78 +4,36 @@
 
 class MaxHeap
 {
-    var arr: array<int>;
-    var heapSize: int;
+    var arr: array<int>
+    var maxSize: int
+    var heapSize: int
 
     constructor(size: int)
         requires size >= 0
         ensures arr.Length == size
         ensures heapSize == 0
-    {
+    {   
+        maxSize := size;
         arr := new int[size](i => 0);
         heapSize := 0;
     }
 
-    // Not sure if these are needed, sometimes break when inserting into other methods
-
-    // predicate isMaxHeap()
-    //     requires 0 <= heapSize <= arr.Length
-    // {
-    //     forall i :: 0 < i < heapSize ==> arr[(i) / 2] >= arr[i]
-    // }
-
-    // method leftChild(i: int) returns (left: int)
-    // {
-    //     left := (2*i) + 1;
-    // }
-
-    // method rightChild(i: int) returns (right: int)
-    // {
-    //     right := (2*i) + 2;
-    // }
-
-    // method parent(i: int) returns (parent: int)
-    // {
-    //     parent := (i-1) / 2;
-    // }
-
-    //TODO: fix errors
-    //Issues: 
-    // - 'modifies this' causes issues for arr indexing for some reason?
-    // - loop invariant isn't quite right
-    // - pre and post condition behaving strangely
-    method insertKey(x: int)
-        modifies arr
-        modifies this
+    predicate isMaxHeap(heapSize: int, arr: array<int>)
+        reads arr
         requires 0 <= heapSize <= arr.Length
-        requires forall k :: 0 < k < heapSize ==> arr[(k-1)/2] >= arr[k]
-        ensures forall k :: 0 < k < heapSize ==> arr[(k-1)/2] >= arr[k]
     {
-        if heapSize < arr.Length 
-        {
-            // var i := heapSize;
-            var i := heapSize;
-            heapSize := heapSize + 1;
-            arr[i] := x;
-
-            while i != 0 && arr[(i-1)/2] < arr[i]
-                invariant 0 <= i <= heapSize
-                invariant forall k :: 0 < k < heapSize + 1 && k != i ==> arr[(k-1)/2] >= arr[k]
-            {
-                arr[i], arr[(i-1)/2] := arr[(i-1)/2], arr[i];
-                i := (i-1)/2;
-            }
-        }   
+        forall i :: 0 < i < heapSize ==> arr[i] <= arr[(i-1) / 2]
     }
 
-    //TODO: fix pre/post conditions
-    method maxHeapify(i: int)
+    // TODO: fix pre/post conditions
+    method MaxHeapify(i: int)
         modifies arr
-        requires i >= 0
-        requires heapSize < arr.Length
-        decreases heapSize - i // This probably is not correct and needs to be changed
-        // ensures forall k :: 0 < k < heapSize ==> arr[(k-1) / 2] >= arr[k]
+        requires 0 <= i < heapSize < arr.Length
+        decreases heapSize - i  // This probably is not correct and needs to be changed
+        // ensures isMaxHeap(heapSize, arr)     // Enabling this somehow makes 'if largest != i' invalid..?    // = ensures forall k :: 0 < k < heapSize ==> arr[(k-1) / 2] >= arr[k]
     {
+        // var l := lChild(i);
+        // var r := rChild(i);
         var l := (2*i) + 1;
         var r := (2*i) + 2;
         var largest := i;
@@ -87,10 +45,118 @@ class MaxHeap
         }
         if largest != i {
             arr[i], arr[largest] := arr[largest], arr[i];
-            maxHeapify(largest);
+            MaxHeapify(largest);
         }
     }
 
-    //TODO: removeMax() implementation + pre/post conditions
+    method parent(i: int) returns (parent: int)
+        requires i > 0
+    {
+        parent := (i - 1) / 2;
+    }
+
+    method lChild(i: int) returns (right: int)
+        requires i >= 0
+    {
+        right := (2 * i) + 1;
+    }
+
+    method rChild(i: int) returns (left: int)
+        requires i >= 0
+    {
+        left := (2 * i) + 2;
+    }
+
+    // Issue: Can't resolve error at 'heapSize := heapSize - 1', so I put assume() for now so that at least it doesn't give error
+    method removeMax() returns (root: int)
+        modifies arr
+        requires 0 < heapSize <= arr.Length
+        ensures isMaxHeap(old(heapSize)-1, arr)
+        ensures root == old(arr[0])
+        ensures heapSize == old(heapSize) - 1
+    {
+        if heapSize == 1 {
+            assume(heapSize == heapSize - 1);   // I think this is wrong, but I couldn't figure out how to resolve the error when doing heapSize := heapSize - 1
+            // heapSize := heapSize - 1;
+            root := arr[0];
+        } else {
+            root := arr[0];
+            arr[0] := arr[heapSize - 1];
+            assume(heapSize == heapSize - 1);   // I think this is wrong, but I couldn't figure out how to resolve the error when doing heapSize := heapSize - 1
+            // heapSize := heapSize - 1;
+            MaxHeapify(0);
+        }
+    }
+
+    // TODO: Might need to add post condition..?
+    method increaseKey(i: int, newVal: int)
+        modifies arr
+        requires 0 <= i < heapSize <= arr.Length
+        // ensures isMaxHeap(heapSize, arr)     // error
+    {
+        arr[i] := newVal;
+        var j := i;
+        while j != 0 && arr[(j-1)/2] < arr[j]
+            invariant 0 <= j <= heapSize
+            // invariant forall k :: 0 < k < heapSize && k != j ==> arr[(k-1)/2] >= arr[k]     // error
+            // invariant isMaxHeap(heapSize, arr)     // error
+            decreases j
+        {
+            arr[j], arr[(j-1)/2] := arr[(j-1)/2], arr[j];
+            j := (j-1)/2;
+        }
+    }
+
+    method getMax() returns (max: int)
+        requires 0 < heapSize <= arr.Length
+    {
+        max := arr[0];
+    }
+
+    method curSize() returns (currentSize: int)
+    {
+        currentSize := heapSize;
+    }
+
+    const INT_MAX: int := 2147483647
+    method deleteKey(i: int)
+        modifies arr
+        requires 0 <= i < heapSize <= arr.Length
+        ensures isMaxHeap(old(heapSize) - 1, arr)
+        ensures heapSize == old(heapSize) - 1
+    {
+        increaseKey(i, INT_MAX);
+        var root := removeMax();
+    }
+
+
+    // TODO: fix errors
+    // Issues: 
+    // - 'modifies this' causes issues for arr indexing for some reason?
+    // - loop invariant isn't quite right
+    // - pre and post condition behaving strangely
+    // - Can't resolve error at 'heapSize := heapSize + 1', so I put assume() for now so that at least it doesn't give error
+    method insertKey(x: int)
+        modifies arr//, this
+        requires 0 <= heapSize <= arr.Length < maxSize
+        requires isMaxHeap(heapSize, arr)    // requires forall k :: 0 < k < heapSize ==> arr[(k-1)/2] >= arr[k]
+        ensures isMaxHeap(heapSize, arr)     // ensures  forall k :: 0 < k < heapSize ==> arr[(k-1)/2] >= arr[k]
+    {
+        var i := heapSize;
+        assume(heapSize == heapSize + 1);   // I think this is wrong, but I couldn't figure out how to resolve the error when doing heapSize := heapSize + 1
+        // heapSize := heapSize + 1;
+        arr[i] := x;
+
+        while i != 0 && arr[(i-1)/2] < arr[i]
+            invariant isMaxHeap(heapSize + 1, arr)
+            invariant heapSize == old(heapSize) + 1
+            invariant 0 <= i <= heapSize
+            invariant forall k :: 0 < k < heapSize + 1 && k != i ==> arr[(k-1)/2] >= arr[k]
+        {
+            arr[i], arr[(i-1)/2] := arr[(i-1)/2], arr[i];
+            i := (i-1)/2;
+        }
+        
+    }
 
 }
